theories/Itauto.v
@@ -51,6 +51,8 @@ Ltac itauto tac  :=
   | false => vitautog
   end.
 
+Ltac itautor tac := let t := solve[tac | itauto tac] in itauto t.
+
 Ltac smt :=
   let tac := no congruence lia in
   (* zify of div mod generate propositional formulae *)
@@ -58,3 +60,51 @@ Ltac smt :=
 
 Ltac Zify.zify_convert_to_euclidean_division_equations_flag ::= constr:(false).
 Ltac Zify.zify_post_hook ::= idtac. (* ZifyBool sets some nasty Ltac *)
+
+Module Redef.
+
+  (* old tauto and intuition *)
+  Ltac otauto := tauto.
+  Tactic Notation "ointuition" tactic(t) := intuition t.
+
+  (* Emulate intuition and tauto *)
+  Ltac nneg :=
+    match goal with
+    | H1 : (?T1 -> False) |- False => apply H1 ; assumption
+    end.
+
+  Ltac tauto_solve :=
+    solve[reflexivity| assumption | nneg].
+
+  Ltac tautor :=
+    let t := solve [tauto_solve|itauto tauto_solve] in
+    itauto t.
+
+  Ltac tauto := itauto tauto_solve.
+
+  Tactic Notation "intuition" tactic(t) :=
+    itauto t.
+
+  Ltac intuitionr t :=
+    let tac := solve[t |itauto t] in
+    itauto tac.
+
+
+End Redef.
+
+Module Bench.
+
+  Lemma double : forall (P:Prop), P -> P -> P.
+  Proof.
+    auto.
+  Qed.
+
+  Ltac apply_double :=
+    match goal with
+    | |- ?G => apply (double G)
+    end.
+
+  Ltac tac_or_tac t1 t2 :=
+    solve [apply_double ; [solve [ time "T1" t1] | solve [time "T2" t2]]].
+
+End Bench.
